\left(\forall_{a_{1}, b_{1}~|~a_{1} = b_{1}}~\left(\left(a_{1}\right) = \left(b_{1}\right)\right) , \forall_{m \in \mathbb{N}^+~|~\forall_{a_{1},\ldots,a_{m}, b_{1},\ldots,b_{m}~|~a_{1} = b_{1} , \ldots , a_{m} = b_{m}}~\left(\left(a_{1} , \ldots , a_{m}\right) = \left(b_{1} , \ldots , b_{m}\right)\right)}~\left[\forall_{a_{1},\ldots,a_{m + 1}, b_{1},\ldots,b_{m + 1}~|~a_{1} = b_{1} , \ldots , a_{m + 1} = b_{m + 1}}~\left(\left(a_{1} , \ldots , a_{m + 1}\right) = \left(b_{1} , \ldots , b_{m + 1}\right)\right)\right]\right)